Common/HashSet.lean
@@ -1,9 +1,123 @@
 import Std.Data.HashSet
 import Common.Finite
 
+
 open Std.HashSet
 namespace Std.HashSet
 
-theorem finite_size {α : Type u} [Finite α] [BEq α] [LawfulBEq α] [Hashable α] (set : Std.HashSet α) : set.size ≤ Finite.cardinality α := by
+theorem erase_not_mem {α : Type u} [BEq α] [Hashable α] [LawfulBEq α] (set : HashSet α) (a : α) : a ∉ (set.erase a) := by
+  simp only [HashSet.mem_iff_contains, HashSet.contains_erase, beq_self_eq_true, Bool.not_true, Bool.false_and, Bool.false_eq_true, not_false_eq_true]
 
-  sorry
+theorem erase_not_mem_of_not_mem {α : Type u} [BEq α] [Hashable α] [LawfulBEq α] (set : HashSet α) {a : α} (b : α) (h₁ : a ∉ set) : a ∉ (set.erase b) := by
+  intro h₂
+  rw[HashSet.mem_erase] at h₂
+  exact absurd h₂.right h₁
+
+protected theorem size_le_finite_worker_size (α : Type u) [Finite α] [BEq α] [Hashable α] [LawfulBEq α] : ∀ (set : Std.HashSet α) (n : Fin (Finite.cardinality α)) (_h₁ : ∀(o : Fin (Finite.cardinality α)) (_h : o > n), Finite.nth o ∉ set), set.size ≤ (Finite.set.set_worker α HashSet.empty  n).size := by
+  intros set n h₁
+  cases n
+  case mk n h₂ =>
+  cases n
+  case zero =>
+    have h₃ : (Finite.set.set_worker α empty ⟨0,h₂⟩).size = 1 := by simp[Finite.set.set_worker, HashSet.size_insert]
+    rw[h₃]
+    cases h₄ : set.contains (Finite.nth ⟨0,h₂⟩)
+    case false =>
+      have h₅ : ∀(o : Fin (Finite.cardinality α)), Finite.nth o ∉ set := by
+        simp[←Bool.not_eq_true, ←HashSet.mem_iff_contains] at h₄
+        intro o
+        cases o
+        case mk o ho =>
+        cases o
+        case zero => exact h₄
+        case succ oo => exact h₁ ⟨oo+1, ho⟩ (Nat.succ_pos oo)
+      have h₆ : ∀(a : α), a∉set := Finite.forall_nth (λx ↦ x∉set) h₅
+      have h₇ : set.isEmpty = true := HashSet.isEmpty_iff_forall_not_mem.mpr h₆
+      have h₈ : true = (set.size == 0) := HashSet.isEmpty_eq_size_eq_zero.subst h₇.symm
+      have h₈ : set.size = 0 := beq_iff_eq.mp h₈.symm
+      rw[h₈]
+      exact Nat.zero_le _
+    case true =>
+      --show that the set from which we erase (nth 0) has size 0, just like in case false.
+      --then show that, since we removed one element, set.size equals 1.
+      let rset := set.erase $ Finite.nth ⟨0,h₂⟩
+      have h₅ : (Finite.nth ⟨0,h₂⟩) ∉ rset := erase_not_mem set (Finite.nth ⟨0,h₂⟩)
+      have h₆ : ∀(o : Fin (Finite.cardinality α)), Finite.nth o ∉ rset := by
+        intro o
+        cases o
+        case mk o ho =>
+        cases o
+        case zero => exact h₅
+        case succ oo => exact erase_not_mem_of_not_mem set _ $ h₁ ⟨oo+1, ho⟩ (Nat.succ_pos oo)
+      have h₇ : ∀(a : α), a∉rset := Finite.forall_nth (λx ↦ x∉rset) h₆
+      have h₈ : rset.isEmpty = true := HashSet.isEmpty_iff_forall_not_mem.mpr h₇
+      have h₉ : true = (rset.size == 0) := HashSet.isEmpty_eq_size_eq_zero.subst h₈.symm
+      have h₉ : rset.size = 0 := beq_iff_eq.mp h₉.symm
+      have h₁₀ : set.size ≤ rset.size + 1 := HashSet.size_le_size_erase
+      rw[h₉, Nat.zero_add] at h₁₀
+      assumption
+  case succ m =>
+    --erase (nth m) from the set and recurse.
+    --then show that the current set can only be larger by 1, and therefore fulfills the goal
+    --HashSet.size_le_size_erase
+    let rset := set.erase $ Finite.nth ⟨m+1,h₂⟩
+    have h₃ : (Finite.nth ⟨m+1,h₂⟩) ∉ rset := erase_not_mem set (Finite.nth ⟨m+1,h₂⟩)
+    have h₄ : ∀(o : Fin (Finite.cardinality α)) (h₄ : o > ⟨m,Nat.lt_of_succ_lt h₂⟩), Finite.nth o ∉ rset := by
+      intros o h₄
+      cases o
+      case mk o h₅ =>
+      cases h₆ : o == (m+1) <;> simp at h₆
+      case true =>
+        simp only[h₆]
+        exact erase_not_mem set $ Finite.nth ⟨m+1, h₂⟩
+      case false =>
+        have h₆ : o > m+1 := by simp at h₄; omega
+        exact erase_not_mem_of_not_mem _ _ (h₁ ⟨o,h₅⟩ h₆)
+    have h₅ := Std.HashSet.size_le_finite_worker_size α rset ⟨m, Nat.lt_of_succ_lt h₂⟩ h₄
+    have h₆ : (Finite.set.set_worker α empty ⟨m, Nat.lt_of_succ_lt h₂⟩).size = empty.size + m + 1 :=
+      Finite.set_worker_size α empty ⟨m, Nat.lt_of_succ_lt h₂⟩ (λa _ ↦Bool.eq_false_iff.mp $ HashSet.contains_empty (a := Finite.nth a))
+    have h₇ : (Finite.set.set_worker α empty ⟨m+1,h₂⟩).size = empty.size + (m + 1) + 1 :=
+      Finite.set_worker_size α empty ⟨m+1,h₂⟩ (λa _ ↦Bool.eq_false_iff.mp $ HashSet.contains_empty (a := Finite.nth a))
+    have h₈ := HashSet.size_le_size_erase (m := set) (k:=Finite.nth ⟨m+1,h₂⟩)
+    simp[h₆] at h₅
+    simp[h₇]
+    exact Nat.le_trans h₈ (Nat.succ_le_succ h₅)
+
+theorem size_le_finite_set_size {α : Type u} [Finite α] [BEq α] [LawfulBEq α] [Hashable α] (set : Std.HashSet α) : set.size ≤ (Finite.set α).size := by
+  unfold Finite.set
+  split
+  case h_1 h₁ =>
+    if h : set.isEmpty then
+      have := HashSet.isEmpty_eq_size_eq_zero (m := set)
+      simp[h] at this
+      simp[this]
+    else
+      have := HashSet.isEmpty_eq_false_iff_exists_mem.mp (Bool.eq_false_iff.mpr h)
+      cases this
+      case intro x hx =>
+        let xx := Finite.enumerate x
+        exact (Fin.cast h₁ xx).elim0
+  case h_2 l h =>
+    exact Std.HashSet.size_le_finite_worker_size α set ⟨l,h.substr $ Nat.lt_succ_self l⟩ (λa hx ↦
+      by
+      have h₁ := a.isLt
+      simp_arith[h] at h₁
+      have h₂ : a > l := Fin.lt_iff_val_lt_val.mp hx
+      exact absurd h₁ (Nat.not_le.mpr h₂)
+    )
+
+theorem size_le_finite_cardinality {α : Type u} [Finite α] [BEq α] [LawfulBEq α] [Hashable α] (set : Std.HashSet α) : set.size ≤ Finite.cardinality α :=
+  (Finite.set_size_eq_cardinality α).subst (size_le_finite_set_size set)
+
+theorem size_lt_finite_cardinality_of_not_mem {α : Type u} [Finite α] [BEq α] [LawfulBEq α] [Hashable α] (set : Std.HashSet α) (h₁ : ∃(a : α), a ∉ set) : set.size < Finite.cardinality α := by
+  have h₂ : set.size ≤ Finite.cardinality α := size_le_finite_cardinality set
+  cases h₁
+  case intro e h₁ =>
+  let iset := set.insert e
+  have h₂ : iset.size = set.size + 1 := by
+    have := HashSet.size_insert (m := set) (k := e)
+    simp[h₁] at this
+    assumption
+  have h₃ : iset.size ≤ Finite.cardinality α := size_le_finite_cardinality iset
+  rw[h₂] at h₃
+  exact Nat.lt_of_succ_le h₃
